Qed ctr.client.MakeClerk.

src/program_proof/fencing/client_proof.v
@@ -14,21 +14,67 @@ Context `{!heapGS Σ}.
 Record client_names :=
   {
     config_gn: config.names;
+    kv_gn : gname;
   }.
 
 Implicit Type γ : client_names.
 Context `{!urpcregG Σ}.
+Context `{!ctrG Σ}.
+
+Definition config_host_inv γ (host:u64) : iProp Σ :=
+  ∃ γfe,
+  ⌜γfe.(frontend.kv_gn) = γ.(kv_gn)⌝ ∗
+  frontend.is_host γfe host.
 
 (* This is "own" not "is" because the frontendCk field is written to inside of
    FetchAndIncrement, so it's actually not safe for one Clerk to have concurrent
    FAIs. *)
 Definition own_Clerk γ ck : iProp Σ :=
-  ∃ (configCk frontendCk:loc),
+  ∃ (configCk frontendCk:loc) γfe,
   "HconfigCk" ∷ ck ↦[client.Clerk :: "configCk"] #configCk ∗
   "HfrontendCk" ∷ ck ↦[client.Clerk :: "frontendCk"] #frontendCk ∗
 
-  "HconfigCk_own" ∷ config.is_Clerk γ.(config_gn) configCk (λ _, True) (λ _, True)
+  "#HconfigCk_is" ∷ config.is_Clerk γ.(config_gn) configCk (λ _, True) (config_host_inv γ) ∗
+  "#HfrontendCk_is" ∷ frontend.is_Clerk γfe frontendCk ∗
+  "%Hfrontend_gn" ∷ ⌜γfe.(frontend.kv_gn) = γ.(kv_gn)⌝
 .
+
+Lemma wp_MakeClerk γ configHost :
+  config.is_host γ.(config_gn) configHost (λ _, True) (config_host_inv γ) -∗
+  {{{
+        True
+  }}}
+    client.MakeClerk #configHost
+  {{{
+        (ck:loc), RET #ck; own_Clerk γ ck
+  }}}
+.
+Proof.
+  iIntros "#Hcfg !#" (Φ) "_ HΦ".
+  wp_call.
+  wp_apply (wp_allocStruct).
+  { repeat econstructor. }
+  iIntros (ck) "Hck".
+  wp_pures.
+
+  iDestruct (struct_fields_split with "Hck") as "HH".
+  iNamed "HH".
+  wp_apply (config.wp_MakeClerk with "Hcfg").
+  iIntros (configCk) "#HconfigCk_is".
+  wp_storeField.
+  wp_loadField.
+  wp_apply (config.wp_Clerk__Get with "HconfigCk_is").
+  iIntros (frontendHost) "#HfrontendHost".
+  iDestruct "HfrontendHost" as (?) "[%Hfe_gn #HfrontendHost]".
+  wp_pures.
+  wp_apply (frontend.wp_MakeClerk with "HfrontendHost").
+  iIntros (frontendCk) "#HfrontendCk_is".
+  wp_storeField.
+  iApply "HΦ".
+  iExists _, _, _.
+  iFrame "∗#".
+  done.
+Qed.
 
 End client_proof.
 End client.
